increment pointer by one

c/poc/strlen.c
@@ -1,16 +1,11 @@
 typedef unsigned int size_t;
 
-size_t strlen(const unsigned char *s) {
-  size_t i;
-  unsigned char c;
+size_t strlen(const unsigned char *s)
+{
+  size_t i = 0;
 
-  i = 0;
-  c = s[i];
-  while ('\0' != c) {
-    i++;
-    c = s[i];
-    
-  }
+  while(*s++)
+      i++;
 
   return i;
 }
